src/dvspec/dafny/implementation/dvc_implementation.dfy
@@ -1,39 +1,63 @@
 include "../commons.dfy"
+
 abstract module DVCNode_Implementation
 {
     import opened Types
     import opened CommonFunctions
-    import opened DVCNode_Externs: DVCNode_Externs
+    import opened DVCNode_Externs : DVCNode_Externs
 
     export PublicInterface
-        reveals DVCNode,
-                AttestationSignatureShareDB
+        reveals DVCNode        
         provides
                 DVCNode.serve_attestation_duty, 
                 DVCNode.att_consensus_decided, 
                 DVCNode.listen_for_attestation_shares,
                 DVCNode.listen_for_new_imported_blocks,
                 DVCNode.resend_attestation_share,
-                DVCNode.bn
+                DVCNode.bn,
+                DVCNode.att_consensus,
+                DVCNode.network
         provides Types, DVCNode_Externs
 
-    type AttestationSignatureShareDB = map<(AttestationData, seq<bool>), set<AttestationShare>>   
+    class AttestationConsensusValidityCheck extends ConsensusValidityCheck<AttestationData>
+    {
+        const dvcNode: DVCNode
+        const attestation_duty: AttestationDuty
+
+        constructor(
+            dvcNode: DVCNode,
+            attestation_duty: AttestationDuty
+        )
+        ensures this.dvcNode == dvcNode
+        ensures this.attestation_duty == attestation_duty
+        {
+            this.dvcNode := dvcNode;
+            this.attestation_duty := attestation_duty;
+        }
+
+        predicate is_valid(data: AttestationData)
+        reads *
+        {
+            consensus_is_valid_attestation_data(dvcNode.attestation_slashing_db, data, this.attestation_duty)             
+        }
+    }
 
     class DVCNode {
 
         var current_attesation_duty: Optional<AttestationDuty>;
+        var latest_attestation_duty: Optional<AttestationDuty>;
         var attestation_duties_queue: seq<AttestationDuty>;
         // var pubkey: BLSPubkey;
         var attestation_slashing_db: AttestationSlashingDB;
         var attestation_shares_db: AttestationSignatureShareDB;
-        var attestation_share_to_broadcast: Optional<AttestationShare>
+        var attestation_shares_to_broadcast: map<Slot, AttestationShare>
         var construct_signed_attestation_signature: (set<AttestationShare>) -> Optional<BLSSignature>;
         var peers: set<BLSPubkey>;
         // TODO: Note difference with spec.py
         var dv_pubkey: BLSPubkey;
         var future_att_consensus_instances_already_decided: set<Slot>
 
-        var att_consensus: Consensus;
+        var att_consensus: Consensus<AttestationData>;
         const network : Network
         const bn: BeaconNode;
         const rs: RemoteSigner;
@@ -41,15 +65,17 @@ abstract module DVCNode_Implementation
         constructor(
             pubkey: BLSPubkey, 
             dv_pubkey: BLSPubkey,
-            att_consensus: Consensus, 
+            att_consensus: Consensus<AttestationData>, 
             peers: set<BLSPubkey>,
             network: Network,
             bn: BeaconNode,
             rs: RemoteSigner,
-            construct_signed_attestation_signature: (set<AttestationShare>) -> Optional<BLSSignature>)
+            construct_signed_attestation_signature: (set<AttestationShare>) -> Optional<BLSSignature>
+        )
         {
             current_attesation_duty := None;
-            attestation_share_to_broadcast := None;
+            latest_attestation_duty := None;
+            attestation_shares_to_broadcast := map[];
             attestation_shares_db := map[];
 
             // this.pubkey := pubkey;
@@ -65,15 +91,19 @@ abstract module DVCNode_Implementation
 
         method serve_attestation_duty(
             attestation_duty: AttestationDuty
-        )
-        modifies this
+        ) returns (s: Status)
+        modifies this, this.att_consensus
         {
             attestation_duties_queue := attestation_duties_queue + [attestation_duty];
-            check_for_next_queued_duty();
+            {
+                :- check_for_next_queued_duty();
+            }
+
+            return Success;
         }
 
-        method check_for_next_queued_duty()
-        modifies this
+        method check_for_next_queued_duty() returns (s: Status)
+        modifies this, this.att_consensus
         decreases attestation_duties_queue
         {
             if attestation_duties_queue != []
@@ -81,33 +111,34 @@ abstract module DVCNode_Implementation
                 if attestation_duties_queue[0].slot in future_att_consensus_instances_already_decided
                 {
                     attestation_duties_queue := attestation_duties_queue[1..];
-                    check_for_next_queued_duty();
+                    { :- check_for_next_queued_duty();}
                 }
                 else if !current_attesation_duty.isPresent()
                 {
                     var queue_head := attestation_duties_queue[0];
                     attestation_duties_queue := attestation_duties_queue[1..];
 
-                    start_next_duty(queue_head);
+                    :- start_next_duty(queue_head);
                 }
             }
+
+            return Success;
         }
 
-        method start_next_duty(attestation_duty: AttestationDuty)
-        modifies this
+        method start_next_duty(attestation_duty: AttestationDuty) returns (s: Status)
+        modifies this, this.att_consensus
         {
             attestation_shares_db := map[];
-            attestation_share_to_broadcast := None;
             current_attesation_duty := Some(attestation_duty);
-            att_consensus.start(attestation_duty.slot);            
+            latest_attestation_duty := Some(attestation_duty);
+            var validityCheck := new AttestationConsensusValidityCheck(this, attestation_duty);
+            { :- att_consensus.start(attestation_duty.slot, validityCheck);}
+            return Success;
         }        
 
         method update_attestation_slashing_db(attestation_data: AttestationData, attestation_duty_pubkey: BLSPubkey)
-        modifies this       
+        modifies this`attestation_slashing_db
         {
-            // assert not is_slashable_attestation_data(attestation_slashing_db, attestation_data, pubkey)
-            // TODO: Is the following required given that each co-validator only handles one pubkey?
-            // slashing_db_data = get_slashing_db_data_for_pubkey(attestation_slashing_db, pubkey)
             var slashing_db_attestation := SlashingDBAttestation(
                                                 source_epoch := attestation_data.source.epoch,
                                                 target_epoch := attestation_data.target.epoch,
@@ -119,23 +150,27 @@ abstract module DVCNode_Implementation
             id: Slot,
             decided_attestation_data: AttestationData
         ) returns (r: Status)
-        modifies this
+        modifies this, this.network, this.att_consensus
         {
-            var local_current_attestation_duty :- current_attesation_duty.get();
+            var local_current_attestation_duty :- current_attesation_duty.get();            
             update_attestation_slashing_db(decided_attestation_data, local_current_attestation_duty.pubkey);
  
             var fork_version := bn.get_fork_version(compute_start_slot_at_epoch(decided_attestation_data.target.epoch));
             var attestation_signing_root := compute_attestation_signing_root(decided_attestation_data, fork_version);
             var attestation_signature_share := rs.sign_attestation(decided_attestation_data, fork_version, attestation_signing_root);
-            // TODO: What is attestation_signature_share.aggregation_bits?
             var attestation_with_signature_share := AttestationShare(
                 aggregation_bits := get_aggregation_bits(local_current_attestation_duty.validator_index),
                 data := decided_attestation_data, 
                 signature :=attestation_signature_share
             ); 
 
-            attestation_share_to_broadcast := Some(attestation_with_signature_share);
-            network.send_att_share(attestation_with_signature_share, peers);           
+            attestation_shares_to_broadcast := attestation_shares_to_broadcast[local_current_attestation_duty.slot := attestation_with_signature_share];
+            network.send_att_share(attestation_with_signature_share, peers);  
+            current_attesation_duty := None;
+            
+            { :- check_for_next_queued_duty(); }
+
+            return Success;         
         }
 
         function method get_aggregation_bits(
@@ -150,7 +185,7 @@ abstract module DVCNode_Implementation
         method listen_for_attestation_shares(
             attestation_share: AttestationShare
         )
-        modifies this
+        modifies this, this.bn
         {
             // TODO: Decide 
             // 1. whether to add att shares to db only if already served attestation duty
@@ -177,51 +212,57 @@ abstract module DVCNode_Implementation
         method listen_for_new_imported_blocks(
             block: BeaconBlock
         ) returns (s: Status)
-        modifies this
+        modifies this, this.att_consensus
         {
             var valIndex :- bn.get_validator_index(block.body.state_root, dv_pubkey);
             var i := 0;
 
+            var att_consensus_instances_already_decided := future_att_consensus_instances_already_decided;
+
             while i < |block.body.attestations|
-            // for i := 0 to |block.body.attestations|
             {
                 var a := block.body.attestations[i];
+
                 var committee :- bn.get_epoch_committees(block.body.state_root, a.data.index);
                 
                 if
                 && a in block.body.attestations
-                // && a.data.slot == process.attestation_duty.slot 
-                // && a.data.index == process.attestation_duty.committee_index
                 && valIndex.Some?
                 && valIndex.v in committee
                 && var i:nat :| i < |committee| && committee[i] == valIndex.v;
                 && i < |a.aggregation_bits|
                 && a.aggregation_bits[i]
-                && (current_attesation_duty.isPresent() ==> a.data.slot >= current_attesation_duty.safe_get().slot)
                 {
-                    future_att_consensus_instances_already_decided := future_att_consensus_instances_already_decided + {a.data.slot};
+                    att_consensus_instances_already_decided := att_consensus_instances_already_decided + {a.data.slot};
                 }
 
                 i := i + 1;
             }
 
+            att_consensus.stop_multiple(att_consensus_instances_already_decided);
+            attestation_shares_to_broadcast := attestation_shares_to_broadcast - att_consensus_instances_already_decided;
 
-            if current_attesation_duty.isPresent() && current_attesation_duty.safe_get().slot in future_att_consensus_instances_already_decided
+            if latest_attestation_duty.isPresent()
             {
-                att_consensus.stop(current_attesation_duty.safe_get().slot);
-                current_attesation_duty := None;
-                check_for_next_queued_duty();
-            }                                   
+                future_att_consensus_instances_already_decided := 
+                        set i | 
+                            && i in att_consensus_instances_already_decided 
+                            && i > latest_attestation_duty.safe_get().slot
+                        ;
+            }
+            else
+            {
+                future_att_consensus_instances_already_decided := att_consensus_instances_already_decided;
+            }
+
+            return Success;                              
         }
 
         method resend_attestation_share(
         )
-        modifies this
+        modifies this, this.network
         {
-            if attestation_share_to_broadcast.isPresent()
-            {
-                network.send_att_share(attestation_share_to_broadcast.safe_get(), peers);
-            }
+            network.send_att_shares(attestation_shares_to_broadcast.Values, peers);
         }        
     }    
 }
@@ -231,56 +272,54 @@ module DVCNode_Externs
     import opened Types
     import opened CommonFunctions
 
-    class Consensus {
-        ghost var consensus_commands_sent: seq<ConsensusCommand>
+    trait Consensus<T(!new, ==)>
+    {
+        ghost var consensus_instances_started: map<Slot, ConsensusValidityCheck<T>>
 
-        constructor()
-        {
-            consensus_commands_sent := [];
-        }
+        method start(
+            id: Slot,
+            validityPredicate: ConsensusValidityCheck<T>
+        ) returns (s: Status)
+        modifies this
+        requires validityPredicate as object != this
+        ensures s.Success? <==> id !in old(consensus_instances_started.Keys)
+        ensures s.Success? ==> consensus_instances_started == old(consensus_instances_started)[id := validityPredicate]
+        ensures s.Failure? ==> consensus_instances_started == old(consensus_instances_started)       
 
-        method {:extern} start(
-            id: Slot
+        method stop_multiple(
+            ids: set<Slot>
         )
-        ensures consensus_commands_sent == old(consensus_commands_sent) + [ConsensusCommand.Start(id)]
+        modifies this
+        ensures consensus_instances_started == old(consensus_instances_started) - ids
+    }    
 
-        method {:extern} stop(
-            id: Slot
-        )
-        ensures consensus_commands_sent == old(consensus_commands_sent) + [ConsensusCommand.Stop(id)]        
-    }     
-
-    class Network  
+    trait Network  
     {
         ghost var att_shares_sent: seq<set<MessaageWithRecipient<AttestationShare>>>;
 
-        constructor()
-        {
-            att_shares_sent := [];
-        }
-
-        method {:extern} send_att_share(att_share: AttestationShare, receipients: set<BLSPubkey>)
+        method send_att_share(att_share: AttestationShare, receipients: set<BLSPubkey>)
+        modifies this
         ensures att_shares_sent == old(att_shares_sent)  + [addRecepientsToMessage(att_share, receipients)]
+
+        method send_att_shares(att_shares: set<AttestationShare>, receipients: set<BLSPubkey>)
+        modifies this
+        ensures     var setWithRecipient := set att_share | att_share in att_shares :: addRecepientsToMessage(att_share, receipients);
+                    att_shares_sent == old(att_shares_sent)  + [setUnion(setWithRecipient)]
     }
 
-    class BeaconNode
+    trait BeaconNode
     {
         ghost var state_roots_of_imported_blocks: set<Root>;
         ghost const attestations_submitted: seq<Attestation>; 
 
-        constructor()
-        {
-            attestations_submitted := [];
-            state_roots_of_imported_blocks := {};
-        }
+        method get_fork_version(s: Slot) returns (v: Version)
 
-        method {:extern} get_fork_version(s: Slot) returns (v: Version)
-
-        method {:extern} submit_attestation(attestation: Attestation)
+        method submit_attestation(attestation: Attestation)
+        modifies this
         ensures attestations_submitted == old(attestations_submitted) + [attestation]
 
         // https://ethereum.github.io/beacon-APIs/?urls.primaryName=v1#/Beacon/getEpochCommittees
-        method {:extern} get_epoch_committees(
+        method get_epoch_committees(
             state_id: Root,
             index: CommitteeIndex
         ) returns (s: Status, sv: seq<ValidatorIndex>)
@@ -288,25 +327,18 @@ module DVCNode_Externs
         ensures uniqueSeq(sv)  
 
         // https://ethereum.github.io/beacon-APIs/#/Beacon/getStateValidator
-        method {:extern} get_validator_index(
+        method get_validator_index(
             state_id: Root,
             validator_id: BLSPubkey
         ) returns (s: Status, vi: Optional<ValidatorIndex>)
         ensures state_id in state_roots_of_imported_blocks <==> s.Success?
     }
 
-    class RemoteSigner
+    trait RemoteSigner
     {
         const pubkey: BLSPubkey;
 
-        constructor(
-            pubkey: BLSPubkey
-        )
-        {
-            this.pubkey := pubkey;
-        }
-
-        method {:extern} sign_attestation(
+        method sign_attestation(
             attestation_data: AttestationData, 
             fork_version: Version, 
             signing_root: Root           
