src/dvspec/dafny/proof/dvc_implementation_spec_proof.dfy
@@ -1,23 +1,86 @@
 include "../commons.dfy"
 include "../specification/dvc_spec.dfy"
 
-abstract module DVCNode_Implementation_Proofs refines DVCNode_Implementation
+module DVCNode_Implementation_Proofs refines DVCNode_Implementation
 {
     import opened DVCNode_Spec
     import opened DVCNode_Externs = DVCNode_Externs_Proofs
+
+    function toAttestationConsensusValidityCheckState(
+        acvc: ConsensusValidityCheck<AttestationData>
+    ): AttestationConsensusValidityCheckState
+    requires isAttestationConsensusValidityCheck(acvc)
+    reads acvc, (acvc as AttestationConsensusValidityCheck).dvcNode`attestation_slashing_db
+    {
+        var attestation_duty := (acvc as AttestationConsensusValidityCheck).attestation_duty;
+        var attestation_slashing_db := (acvc as AttestationConsensusValidityCheck).dvcNode.attestation_slashing_db;
+        AttestationConsensusValidityCheckState(
+            attestation_duty := attestation_duty,
+            attestation_slashing_db := attestation_slashing_db,
+            validityPredicate := (ad: AttestationData) => consensus_is_valid_attestation_data(attestation_slashing_db, ad, attestation_duty)
+        )
+    }    
+
+    predicate isAttestationConsensusValidityCheck(
+        cvc: ConsensusValidityCheck<AttestationData>
+    )
+    reads cvc
+    {
+        cvc is AttestationConsensusValidityCheck
+    }
+
+    function toAttestationConsensusValidityCheck(
+        cvc: ConsensusValidityCheck<AttestationData>
+    ): AttestationConsensusValidityCheck
+    requires isAttestationConsensusValidityCheck(cvc)
+    reads cvc
+    {
+        cvc as AttestationConsensusValidityCheck
+    }
+
+    lemma lemmaMapKeysHasOneEntryInItems<K, V>(m: map<K, V>, k: K)  
+    requires k in m.Keys
+    ensures exists i :: i in m.Items && i.0 == k 
+    {
+        assert (k, m[k]) in m.Items;
+    }
+    
+    function get_attestation_consensus_active_instances(
+        m: map<Slot, ConsensusValidityCheck<AttestationData>>
+    ): (r: map<Slot, AttestationConsensusValidityCheckState>)
+    reads m.Values, set v: ConsensusValidityCheck<AttestationData>  | && v in m.Values && isAttestationConsensusValidityCheck(v) :: toAttestationConsensusValidityCheck(v).dvcNode`attestation_slashing_db
+    ensures r.Keys <= m.Keys
+    ensures forall k | k in r.Keys :: isAttestationConsensusValidityCheck(m[k]) && r[k] == toAttestationConsensusValidityCheckState(m[k])
+    {  
+            map it | 
+                        && it in m.Items 
+                        && isAttestationConsensusValidityCheck(it.1)
+                    :: 
+                    it.0 := toAttestationConsensusValidityCheckState(it.1)           
+    }
+
+    function toConsensusEngineState(ce: Consensus<AttestationData>): (r: ConsensusEngineState)
+    reads ce, ce.consensus_instances_started.Values, set v: ConsensusValidityCheck<AttestationData>  | && v in ce.consensus_instances_started.Values && isAttestationConsensusValidityCheck(v) :: toAttestationConsensusValidityCheck(v).dvcNode`attestation_slashing_db
+    {
+        ConsensusEngineState(
+            attestation_consensus_active_instances := get_attestation_consensus_active_instances(ce.consensus_instances_started)   
+        )
+    }
 
     export PublicInterface...
         reveals *
 
     function toDVCNodeState(n: DVCNode): DVCNodeState
-    reads n, n.bn, n.rs
+    reads n, n.bn, n.rs, n.att_consensus, n.att_consensus.consensus_instances_started.Values, set v: ConsensusValidityCheck<AttestationData>  | && v in n.att_consensus.consensus_instances_started.Values && isAttestationConsensusValidityCheck(v) :: toAttestationConsensusValidityCheck(v).dvcNode`attestation_slashing_db
     {
         DVCNodeState(
             current_attesation_duty := n.current_attesation_duty,
+            latest_attestation_duty := n.latest_attestation_duty,
             attestation_duties_queue := n.attestation_duties_queue,
             attestation_slashing_db := n.attestation_slashing_db,
             attestation_shares_db := n.attestation_shares_db,
-            attestation_share_to_broadcast := n.attestation_share_to_broadcast,
+            attestation_shares_to_broadcast := n.attestation_shares_to_broadcast,
+            attestation_consensus_engine_state := toConsensusEngineState(n.att_consensus),
             peers := n.peers,
             construct_signed_attestation_signature := n.construct_signed_attestation_signature,
             dv_pubkey := n.dv_pubkey,
@@ -27,38 +90,14 @@ abstract module DVCNode_Implementation_Proofs refines DVCNode_Implementation
         )
     }
 
-    function seqToSet<T>(s: seq<T>): (r: set<T>)
-    {
-        set e | e in s
-    }
-
     function seqMinusToSet<T>(s1: seq<T>, s2: seq<T>): set<T>
-    // requires s2 <= s1 
-    // ensures seqMinus(s1, s2) + s2 == s1
     {
-        set i | |s2| <= i < |s1| :: s1[i]
-    }
-
-    function seqMinusToOptional<T>(s1: seq<T>, s2: seq<T>): Optional<T>
-    requires s2 <= s1 
-    requires |s1| <= |s2| + 1
-    {
-        if s1 == s2 then
-            None 
+        if |s2| <= |s1| then
+            var seqDiff := s1[|s2|..];
+            assert s2 <= s1 ==> s2 + seqDiff == s1;
+            seqToSet(seqDiff)
         else
-            Some(s1[|s2|])
-    }
-
-
-
-
-
-
-    twostate predicate onlyOneMaxConsensusCommandAndSubmittedAttestation(n: DVCNode)
-    reads n, n.att_consensus, n.bn
-    {
-        && |n.att_consensus.consensus_commands_sent| <= |old(n.att_consensus.consensus_commands_sent)| + 1
-        && |n.bn.attestations_submitted| <= |old(n.bn.attestations_submitted)| + 1
+            {}
     }
 
     twostate function getOutputs(n: DVCNode): (o: Outputs)
@@ -66,15 +105,12 @@ abstract module DVCNode_Implementation_Proofs refines DVCNode_Implementation
     {
         Outputs(
             att_shares_sent :=  setUnion(seqMinusToSet(n.network.att_shares_sent, old(n.network.att_shares_sent))),
-            att_consensus_commands_sent := seqMinusToSet(n.att_consensus.consensus_commands_sent, old(n.att_consensus.consensus_commands_sent)),
             attestations_submitted := seqMinusToSet(n.bn.attestations_submitted, old(n.bn.attestations_submitted))
         )
     }
 
-    
-
     twostate function toDVCNodeStateAndOuputs(n: DVCNode): DVCNodeStateAndOuputs
-    reads n, n.network, n.att_consensus, n.bn, n.rs
+    reads n, n.network, n.att_consensus, n.bn, n.rs, n.att_consensus.consensus_instances_started.Values, set v: ConsensusValidityCheck<AttestationData>  | && v in n.att_consensus.consensus_instances_started.Values && isAttestationConsensusValidityCheck(v) :: toAttestationConsensusValidityCheck(v).dvcNode`attestation_slashing_db
     {
         DVCNodeStateAndOuputs(
             state := toDVCNodeState(n),
@@ -82,70 +118,241 @@ abstract module DVCNode_Implementation_Proofs refines DVCNode_Implementation
         )
     }
 
- 
-
-
-
-
     class DVCNode...
     {
 
-        method update_attestation_slashing_db...
-        ensures f_update_attestation_slashing_db(old(toDVCNodeState(this)).attestation_slashing_db, attestation_data, attestation_duty_pubkey) == this.attestation_slashing_db;  
+        predicate isValid()
+        reads this, this.bn, this.network, this.att_consensus, att_consensus.consensus_instances_started.Values
+        {
+            && (forall vp | vp in att_consensus.consensus_instances_started.Values :: 
+                        && isAttestationConsensusValidityCheck(vp)
+                        && toAttestationConsensusValidityCheck(vp).dvcNode == this
+            )
+            && {this} !! {this.bn} !! {this.network} !! {this.att_consensus} !!att_consensus.consensus_instances_started.Values
+        }
+
+        // TODO: Move to refined class?
+        method process_event(
+            event: Event
+        ) returns (s: Status)
+        modifies this, this.att_consensus, this.bn, this.network
+        ensures (old(isValid()) && f_process_event.requires(old(toDVCNodeState(this)), event)) ==>    
+                && isValid()
+                && f_process_event(old(toDVCNodeState(this)), event) == toDVCNodeStateAndOuputs(this)
+                && s.Success?        
+        {
+            match event {
+                case ServeAttstationDuty(attestation_duty) => 
+                    :- serve_attestation_duty(attestation_duty);
+                case AttConsensusDecided(id, decided_attestation_data) => 
+                    :- att_consensus_decided(id,  decided_attestation_data);
+                case ReceviedAttesttionShare(attestation_share) => 
+                    listen_for_attestation_shares(attestation_share);
+                case ImportedNewBlock(block) => 
+                    :- listen_for_new_imported_blocks(block);
+                case ResendAttestationShares => 
+                    resend_attestation_share();
+                case NoEvent =>
+                    
+            }
+
+            match event {
+                case ServeAttstationDuty(attestation_duty) => 
+                    assert (old(isValid()) && f_process_event.requires(old(toDVCNodeState(this)), event)) ==> 
+                        && f_process_event(old(toDVCNodeState(this)), event) == toDVCNodeStateAndOuputs(this)
+                        && isValid();
+                case AttConsensusDecided(id, decided_attestation_data) => 
+                    assert (old(isValid()) && f_process_event.requires(old(toDVCNodeState(this)), event)) ==> 
+                        && f_process_event(old(toDVCNodeState(this)), event) == toDVCNodeStateAndOuputs(this)
+                        && isValid();                
+                case ReceviedAttesttionShare(attestation_share) => 
+                    assert (old(isValid()) && f_process_event.requires(old(toDVCNodeState(this)), event)) ==> 
+                        && f_process_event(old(toDVCNodeState(this)), event) == toDVCNodeStateAndOuputs(this)
+                        && isValid();                
+                case ImportedNewBlock(block) => 
+                    assert (old(isValid()) && f_process_event.requires(old(toDVCNodeState(this)), event)) ==> 
+                        && f_process_event(old(toDVCNodeState(this)), event) == toDVCNodeStateAndOuputs(this)
+                        && isValid();                
+                case ResendAttestationShares => 
+                    assert (old(isValid()) && f_process_event.requires(old(toDVCNodeState(this)), event)) ==> 
+                        && f_process_event(old(toDVCNodeState(this)), event) == toDVCNodeStateAndOuputs(this)
+                        && isValid();                
+                case NoEvent =>
+                    assert (old(isValid()) && f_process_event.requires(old(toDVCNodeState(this)), event)) ==> 
+                        && f_process_event(old(toDVCNodeState(this)), event) == toDVCNodeStateAndOuputs(this)
+                        && isValid();                
+                    
+            }            
+
+            return Success;
+        }
 
         method serve_attestation_duty...
-        ensures f_serve_attestation_duty(old(toDVCNodeState(this)), attestation_duty) == toDVCNodeStateAndOuputs(this);
+        ensures (old(isValid()) && f_serve_attestation_duty.requires(old(toDVCNodeState(this)), attestation_duty)) ==> 
+                && f_serve_attestation_duty(old(toDVCNodeState(this)), attestation_duty) == toDVCNodeStateAndOuputs(this)
+                && isValid()
+                && s.Success?
         {
             ...;
-            assert f_serve_attestation_duty(old(toDVCNodeState(this)), attestation_duty) == toDVCNodeStateAndOuputs(this);
+            {
+                var o := toDVCNodeState(this);
+                ...;
+                assert o == old(toDVCNodeState(this)).(
+                            attestation_duties_queue := old(toDVCNodeState(this)).attestation_duties_queue + [attestation_duty]
+                        );
+                assert (old(isValid()) && f_serve_attestation_duty.requires(old(toDVCNodeState(this)), attestation_duty)) ==> f_serve_attestation_duty(old(toDVCNodeState(this)), attestation_duty) == toDVCNodeStateAndOuputs(this);
+            }
+
         }
 
         method check_for_next_queued_duty...
-        ensures f_check_for_next_queued_duty(old(toDVCNodeState(this))) == toDVCNodeStateAndOuputs(this);
+        ensures (old(isValid()) && f_check_for_next_queued_duty.requires(old(toDVCNodeState(this))))==> 
+                && f_check_for_next_queued_duty(old(toDVCNodeState(this))) == toDVCNodeStateAndOuputs(this)
+                && isValid()
+                && s.Success?
         {
             if...
             {
                 if...
                 {
+
                     ...;
-                    assert f_check_for_next_queued_duty(old(toDVCNodeState(this))) == toDVCNodeStateAndOuputs(this);
+                    {
+                        assert old(isValid()) ==> isValid();
+                        ...;
+
+                        assert (old(isValid()) && f_check_for_next_queued_duty.requires(old(toDVCNodeState(this)))) ==> f_check_for_next_queued_duty(old(toDVCNodeState(this))) == toDVCNodeStateAndOuputs(this);       
+                    }
+
                 }
                 else if...
                 {
                     ...;
-                    assert f_check_for_next_queued_duty(old(toDVCNodeState(this))) == toDVCNodeStateAndOuputs(this);
+                    assert (old(isValid()) && f_check_for_next_queued_duty.requires(old(toDVCNodeState(this)))) ==> f_check_for_next_queued_duty(old(toDVCNodeState(this))) == toDVCNodeStateAndOuputs(this);
                 }
                 else
                 {
-                    assert f_check_for_next_queued_duty(old(toDVCNodeState(this))) == toDVCNodeStateAndOuputs(this);
+                    assert (old(isValid()) && f_check_for_next_queued_duty.requires(old(toDVCNodeState(this)))) ==> f_check_for_next_queued_duty(old(toDVCNodeState(this))) == toDVCNodeStateAndOuputs(this);
                 }
             }
             else
             {
-                assert f_check_for_next_queued_duty(old(toDVCNodeState(this))) == toDVCNodeStateAndOuputs(this);
+                assert (old(isValid()) && f_check_for_next_queued_duty.requires(old(toDVCNodeState(this)))) ==> f_check_for_next_queued_duty(old(toDVCNodeState(this))) == toDVCNodeStateAndOuputs(this);
             }
-
-        }        
+        }     
 
         method start_next_duty...
-        ensures f_start_next_duty(old(toDVCNodeState(this)), attestation_duty) == toDVCNodeStateAndOuputs(this);
+        ensures 
+                old(isValid()) ==>
+                (
+                    && isValid()
+                    && (f_start_next_duty.requires(old(toDVCNodeState(this)), attestation_duty) ==> 
+                        && (f_start_next_duty(old(toDVCNodeState(this)), attestation_duty) == toDVCNodeStateAndOuputs(this))
+                        && s.Success?
+                    )
+                )
         {
+            if old(isValid())
+            {
+                forall e | e in old(att_consensus.consensus_instances_started.Keys)
+                ensures e in old(get_attestation_consensus_active_instances(att_consensus.consensus_instances_started)).Keys; 
+                {
+                    lemmaMapKeysHasOneEntryInItems(old(att_consensus.consensus_instances_started), e);
+                }     
+            }                 
             ...;
-            assert f_start_next_duty(old(toDVCNodeState(this)), attestation_duty) == toDVCNodeStateAndOuputs(this);
+            {
+                ...;
+            }
+            if old(isValid())
+            {
+                lemmaMapKeysHasOneEntryInItems(att_consensus.consensus_instances_started, attestation_duty.slot);
+                                                                                     
+                assert f_start_next_duty(old(toDVCNodeState(this)), attestation_duty) == toDVCNodeStateAndOuputs(this);
+            }
         }
 
-        method att_consensus_decided...
-        ensures old(this.current_attesation_duty).isPresent() ==> f_att_consensus_decided(old(toDVCNodeState(this)), id, decided_attestation_data) == toDVCNodeStateAndOuputs(this);
+        method update_attestation_slashing_db...
+        ensures f_update_attestation_slashing_db(old(toDVCNodeState(this)).attestation_slashing_db, attestation_data, attestation_duty_pubkey) == this.attestation_slashing_db;
+        ensures  var slashing_db_attestation := SlashingDBAttestation(
+                                                source_epoch := attestation_data.source.epoch,
+                                                target_epoch := attestation_data.target.epoch,
+                                                signing_root := Some(hash_tree_root(attestation_data)));
+            attestation_slashing_db == old(attestation_slashing_db) + {slashing_db_attestation};
         {
             ...;
-            if old(this.current_attesation_duty).isPresent()
+        }
+
+        function f_att_consensus_decided_helper(
+            process: DVCNodeState,
+            id: Slot,
+            decided_attestation_data: AttestationData
+        ): DVCNodeStateAndOuputs
+        requires process.current_attesation_duty.isPresent()
+        requires forall ad | ad in process.attestation_duties_queue :: ad.slot !in process.attestation_consensus_engine_state.attestation_consensus_active_instances.Keys    
+        {
+            var local_current_attestation_duty := process.current_attesation_duty.safe_get();
+            var attestation_slashing_db := f_update_attestation_slashing_db(process.attestation_slashing_db, decided_attestation_data, local_current_attestation_duty.pubkey);
+
+            var fork_version := bn_get_fork_version(compute_start_slot_at_epoch(decided_attestation_data.target.epoch));
+            var attestation_signing_root := compute_attestation_signing_root(decided_attestation_data, fork_version);
+            var attestation_signature_share := rs_sign_attestation(decided_attestation_data, fork_version, attestation_signing_root, process.rs);
+            // TODO: What is attestation_signature_share.aggregation_bits?
+            var attestation_with_signature_share := AttestationShare(
+                    aggregation_bits := get_aggregation_bits(local_current_attestation_duty.validator_index),
+                    data := decided_attestation_data, 
+                    signature := attestation_signature_share
+                ); 
+
+            var newProcess := 
+                process.(
+                    current_attesation_duty := None,
+                    attestation_shares_to_broadcast := process.attestation_shares_to_broadcast[local_current_attestation_duty.slot := attestation_with_signature_share],
+                    attestation_slashing_db := attestation_slashing_db,
+                    attestation_consensus_engine_state := updateConsensusInstanceValidityCheck(
+                        process.attestation_consensus_engine_state,
+                        attestation_slashing_db
+                    )
+                )
+                ;
+
+            DVCNodeStateAndOuputs(
+                newProcess,
+                outputs := getEmptyOuputs().(
+                    att_shares_sent := multicast(attestation_with_signature_share, process.peers)
+                )                  
+            )                
+        }        
+
+        method att_consensus_decided...
+        ensures (old(isValid()) && f_att_consensus_decided.requires(old(toDVCNodeState(this)), id, decided_attestation_data)) ==> 
+                && f_att_consensus_decided(old(toDVCNodeState(this)), id, decided_attestation_data) == toDVCNodeStateAndOuputs(this)
+                && isValid()
+                && r.Success?
+        {
+            ...;
             {
-                assert f_att_consensus_decided(old(toDVCNodeState(this)), id, decided_attestation_data) == toDVCNodeStateAndOuputs(this);
+            if old(isValid()) && f_att_consensus_decided.requires(old(toDVCNodeState(this)), id, decided_attestation_data)
+            {
+                var r := f_att_consensus_decided_helper(old(toDVCNodeState(this)), id, decided_attestation_data);
+                var s := old(current_attesation_duty).safe_get().slot;
+
+                forall e | e in old(toDVCNodeState(this)).attestation_consensus_engine_state.attestation_consensus_active_instances.Keys
+                ensures e in r.state.attestation_consensus_engine_state.attestation_consensus_active_instances.Keys
+                {
+                    lemmaMapKeysHasOneEntryInItems(old(toDVCNodeState(this)).attestation_consensus_engine_state.attestation_consensus_active_instances, e);
+                }   
+
+                assert f_att_consensus_decided_helper(old(toDVCNodeState(this)), id, decided_attestation_data).state == toDVCNodeStateAndOuputs(this).state;
+            }                
+                ...;
             }
+            ...;
         }
 
         method listen_for_attestation_shares...
         ensures f_listen_for_attestation_shares(old(toDVCNodeState(this)), attestation_share) == toDVCNodeStateAndOuputs(this);
+        ensures old(isValid()) ==> isValid()
         {
             ...;
         }
@@ -165,32 +372,102 @@ abstract module DVCNode_Implementation_Proofs refines DVCNode_Implementation
                     && isMyAttestation(a, process, block, valIndex)
                 ::
                     a.data.slot
-        }           
+        }  
+
+
+        function listen_for_new_imported_blocks_helper_2(
+            process: DVCNodeState,
+            block: BeaconBlock
+        ): DVCNodeState
+        requires block.body.state_root in process.bn.state_roots_of_imported_blocks
+        {
+        var valIndex := bn_get_validator_index(process.bn, block.body.state_root, process.dv_pubkey);
+         
+        var s := set a |
+                && a in block.body.attestations
+                && isMyAttestation(a, process, block, valIndex)
+            ::
+                a.data.slot;
+
+        var att_consensus_instances_already_decided := process.future_att_consensus_instances_already_decided + s;
+
+        var future_att_consensus_instances_already_decided := 
+                if process.latest_attestation_duty.isPresent() then
+                        set i | 
+                            && i in att_consensus_instances_already_decided 
+                            && i > process.latest_attestation_duty.safe_get().slot
+                else
+                    att_consensus_instances_already_decided
+                        ;
+
+            process.(
+                    // future_att_consensus_instances_already_decided := future_att_consensus_instances_already_decided,
+                    attestation_consensus_engine_state := stopConsensusInstances(
+                                    process.attestation_consensus_engine_state,
+                                    att_consensus_instances_already_decided
+                    ),
+                    attestation_shares_to_broadcast := process.attestation_shares_to_broadcast - att_consensus_instances_already_decided
+            )      
+
+        }   
 
         method listen_for_new_imported_blocks...
-        ensures block.body.state_root in bn.state_roots_of_imported_blocks ==> f_listen_for_new_imported_blocks(old(toDVCNodeState(this)), block) == toDVCNodeStateAndOuputs(this);
+        ensures (old(isValid()) && f_listen_for_new_imported_blocks.requires(old(toDVCNodeState(this)), block)) ==> 
+                    && f_listen_for_new_imported_blocks(old(toDVCNodeState(this)), block) == toDVCNodeStateAndOuputs(this)
+                    && isValid()
+                    && s.Success?
         {
+            assert (old(isValid()) && f_listen_for_new_imported_blocks.requires(old(toDVCNodeState(this)), block)) ==> block.body.state_root in bn.state_roots_of_imported_blocks;
             ...;
             while...
                 invariant 0 <= i <= |block.body.attestations|
-                invariant  block.body.state_root in old(bn.state_roots_of_imported_blocks) ==>
-                    future_att_consensus_instances_already_decided == 
+                invariant  old(isValid()) ==> isValid();                 
+                invariant block.body.state_root in bn.state_roots_of_imported_blocks;
+                invariant (isValid() && block.body.state_root in old(bn.state_roots_of_imported_blocks)) ==>
+                    att_consensus_instances_already_decided == 
                     old(future_att_consensus_instances_already_decided) + listen_for_new_imported_blocks_helper(old(toDVCNodeState(this)), block, valIndex, i); 
                     
-                invariant toDVCNodeState(this) == old(toDVCNodeState(this)).(
-                    future_att_consensus_instances_already_decided := toDVCNodeState(this).future_att_consensus_instances_already_decided
-                )
-                invariant toDVCNodeStateAndOuputs(this).outputs == getEmptyOuputs();            
+                invariant isValid() ==> toDVCNodeState(this) == old(toDVCNodeState(this))
+                invariant toDVCNodeStateAndOuputs(this).outputs == getEmptyOuputs();   
             {
 
+            }
+
+            var o1 := toDVCNodeState(this);
+            ...;
+        
+
+            if...
+            {
+                var o2 := toDVCNodeState(this);
+                assert (old(isValid()) && f_listen_for_new_imported_blocks.requires(old(toDVCNodeState(this)), block)) ==>
+            toDVCNodeState(this) == listen_for_new_imported_blocks_helper_2(old(toDVCNodeState(this)), block);    
+                ...;
+                assert old(isValid()) ==> isValid();
+            }
+            else
+            {
+                var o2 := toDVCNodeState(this);
+                assert (old(isValid()) && f_listen_for_new_imported_blocks.requires(old(toDVCNodeState(this)), block)) ==>
+            toDVCNodeState(this) == listen_for_new_imported_blocks_helper_2(old(toDVCNodeState(this)), block);    
+                ...;
+                assert old(isValid()) ==> isValid();            
             }
         }
 
         method resend_attestation_share...
-        ensures f_resend_attestation_share(old(toDVCNodeState(this))) == toDVCNodeStateAndOuputs(this)
+        ensures old(isValid()) ==>
+                                && isValid()
+                                && f_resend_attestation_share(old(toDVCNodeState(this))) == toDVCNodeStateAndOuputs(this)
         {
             ...;
-            assert  f_resend_attestation_share(old(toDVCNodeState(this))) == toDVCNodeStateAndOuputs(this);
+            assert  old(isValid()) ==> f_resend_attestation_share(old(toDVCNodeState(this))).state == toDVCNodeStateAndOuputs(this).state;
+            var setWithRecipient := set att_share | att_share in attestation_shares_to_broadcast.Values :: addRecepientsToMessage(att_share, peers);
+            var setWithRecipientFlattened := setUnion(setWithRecipient);
+            assert old(isValid()) ==>network.att_shares_sent == old(network.att_shares_sent) +[setWithRecipientFlattened];                
+            assert old(isValid()) ==>seqMinusToSet(network.att_shares_sent, old(network.att_shares_sent)) == {setWithRecipientFlattened};
+            assert  old(isValid()) ==>toDVCNodeStateAndOuputs(this).outputs.att_shares_sent == setWithRecipientFlattened;
+            assert  old(isValid()) ==>f_resend_attestation_share(old(toDVCNodeState(this))) == toDVCNodeStateAndOuputs(this);                  
         }
     }
 }
