src/dvspec/dafny/specification/dvc_spec.dfy
@@ -2,10 +2,9 @@ include "../commons.dfy"
 include "../implementation/dvc_implementation.dfy"
 
 
-abstract module DVCNode_Spec {
+module DVCNode_Spec {
     import opened Types 
     import opened CommonFunctions
-    import opened DVCNode_Implementation`PublicInterface
     import opened DVCNode_Externs
 
     function {:axiom} bn_get_fork_version(slot: Slot): Version
@@ -62,6 +61,91 @@ abstract module DVCNode_Spec {
         pubkey: BLSPubkey
     )
 
+    datatype AttestationConsensusValidityCheckState = AttestationConsensusValidityCheckState(
+        attestation_duty: AttestationDuty,
+        attestation_slashing_db: AttestationSlashingDB,
+        validityPredicate: AttestationData -> bool
+    )
+
+    datatype ConsensusEngineState = ConsensusEngineState(
+        attestation_consensus_active_instances: map<Slot, AttestationConsensusValidityCheckState>
+    )
+
+    function getInitialConensusEngineState(): ConsensusEngineState
+    {
+        ConsensusEngineState(
+            attestation_consensus_active_instances := map[]
+        )
+    }
+
+    // function getValidityPredicate<!T>(
+    //     attestation_slashing_db: AttestationSlashingDB,
+    //     attestation_duty: AttestationDuty
+    // ): T -> bool
+    // {
+    //     (ad: AttestationDuty) => is_valid_attestation_data()
+    // }
+
+    function startConsensusInstance(
+        s: ConsensusEngineState,
+        id: Slot,
+        attestation_duty: AttestationDuty,
+        attestation_slashing_db: AttestationSlashingDB
+    ): ConsensusEngineState
+    requires id !in s.attestation_consensus_active_instances.Keys
+    {
+        var acvc := AttestationConsensusValidityCheckState(
+                    attestation_duty := attestation_duty,
+                    attestation_slashing_db := attestation_slashing_db,
+                    validityPredicate := (ad: AttestationData) => consensus_is_valid_attestation_data(attestation_slashing_db, ad, attestation_duty)
+                );
+        assert (acvc.validityPredicate == (ad: AttestationData) => consensus_is_valid_attestation_data(acvc.attestation_slashing_db, ad, acvc.attestation_duty));
+        s.(
+            attestation_consensus_active_instances := s.attestation_consensus_active_instances[
+                id := acvc
+            ]
+        )
+    }
+
+    function stopConsensusInstances(
+        s: ConsensusEngineState,
+        ids: set<Slot>
+    ): ConsensusEngineState
+    {
+        s.(
+            attestation_consensus_active_instances := s.attestation_consensus_active_instances - ids
+        )
+    }    
+
+    function updateConsensusInstanceValidityCheckHelper(
+        m: map<Slot, AttestationConsensusValidityCheckState>,
+        new_attestation_slashing_db: AttestationSlashingDB
+    ): (r: map<Slot, AttestationConsensusValidityCheckState>)
+    ensures r.Keys <= m.Keys
+    {
+            map it | it in m.Items
+                ::
+                it.0 := it.1.(
+                    attestation_slashing_db := new_attestation_slashing_db,
+                    validityPredicate := (ad: AttestationData) => consensus_is_valid_attestation_data(new_attestation_slashing_db, ad, it.1.attestation_duty)
+                )        
+    }
+
+    function updateConsensusInstanceValidityCheck(
+        s: ConsensusEngineState,
+        new_attestation_slashing_db: AttestationSlashingDB
+    ): (r: ConsensusEngineState)
+    // ensures s.attestation_consensus_active_instances.Keys == r.attestation_consensus_active_instances.Keys
+    {
+        s.(
+            attestation_consensus_active_instances := 
+                updateConsensusInstanceValidityCheckHelper(
+                    s.attestation_consensus_active_instances,
+                    new_attestation_slashing_db
+                )
+        )
+    }
+
     function getInitialRS(
         pubkey: BLSPubkey
     ): RSState
@@ -73,10 +157,13 @@ abstract module DVCNode_Spec {
 
     datatype DVCNodeState = DVCNodeState(
         current_attesation_duty: Optional<AttestationDuty>,
+        latest_attestation_duty: Optional<AttestationDuty>,
         attestation_duties_queue: seq<AttestationDuty>,
         attestation_slashing_db: AttestationSlashingDB,
         attestation_shares_db: AttestationSignatureShareDB,
-        attestation_share_to_broadcast: Optional<AttestationShare>,
+        attestation_shares_to_broadcast: map<Slot, AttestationShare>,
+        attestation_consensus_engine_state: ConsensusEngineState,
+        // attestation_validity_check
         peers: set<BLSPubkey>,
         construct_signed_attestation_signature: (set<AttestationShare>) -> Optional<BLSSignature>,
         // TODO: Note difference with spec.py
@@ -84,11 +171,18 @@ abstract module DVCNode_Spec {
         future_att_consensus_instances_already_decided: set<Slot>,
         bn: BNState,
         rs: RSState
-    )    
+    )
+
+    predicate is_valid_attestation_data(
+        validity_check_data: AttestationConsensusValidityCheckState,
+        attestation_data: AttestationData
+    )
+    {
+        consensus_is_valid_attestation_data(validity_check_data.attestation_slashing_db, attestation_data, validity_check_data.attestation_duty)
+    }
 
     datatype Outputs = Outputs(
         att_shares_sent: set<MessaageWithRecipient<AttestationShare>>,
-        att_consensus_commands_sent: set<ConsensusCommand>,
         attestations_submitted: set<Attestation>
     )    
 
@@ -96,7 +190,7 @@ abstract module DVCNode_Spec {
     {
         Outputs(
             {},
-            {},
+            // {},
             {}
         )
     }  
@@ -106,6 +200,12 @@ abstract module DVCNode_Spec {
     {
         addRecepientsToMessage(m, receipients)
     }
+
+    function multicast_multiple<M>(ms: set<M>, receipients: set<BLSPubkey>): set<MessaageWithRecipient<M>>
+    {
+        var setWithRecipient := set m | m in ms :: addRecepientsToMessage(m, receipients);
+        setUnion(setWithRecipient)
+    }    
 
     datatype DVCNodeStateAndOuputs = DVCNodeStateAndOuputs(
         state: DVCNodeState,
@@ -130,10 +230,12 @@ abstract module DVCNode_Spec {
     {
         s == DVCNodeState(
             current_attesation_duty := None,
+            latest_attestation_duty := None,
             attestation_duties_queue := [],
             attestation_slashing_db := {},
             attestation_shares_db := map[],
-            attestation_share_to_broadcast := None,
+            attestation_shares_to_broadcast := map[],
+            attestation_consensus_engine_state := getInitialConensusEngineState(),
             peers := peers,
             construct_signed_attestation_signature := construct_signed_attestation_signature,
             dv_pubkey := dv_pubkey,
@@ -157,7 +259,8 @@ abstract module DVCNode_Spec {
 
         match event 
             case ServeAttstationDuty(attestation_duty) => 
-                f_serve_attestation_duty(s, attestation_duty) == newNodeStateAndOutputs
+                && f_serve_attestation_duty.requires(s, attestation_duty)
+                && f_serve_attestation_duty(s, attestation_duty) == newNodeStateAndOutputs
             case AttConsensusDecided(id, decided_attestation_data) => 
                 && f_att_consensus_decided.requires(s, id,  decided_attestation_data)
                 && f_att_consensus_decided(s, id,  decided_attestation_data) == newNodeStateAndOutputs
@@ -172,10 +275,45 @@ abstract module DVCNode_Spec {
                 DVCNodeStateAndOuputs(state := s, outputs := getEmptyOuputs() ) == newNodeStateAndOutputs
     }
 
+    function f_process_event(
+        s: DVCNodeState,
+        event: Event
+    ): DVCNodeStateAndOuputs
+    requires
+            match event 
+            case ServeAttstationDuty(attestation_duty) => 
+                && f_serve_attestation_duty.requires(s, attestation_duty)
+            case AttConsensusDecided(id, decided_attestation_data) => 
+                && f_att_consensus_decided.requires(s, id,  decided_attestation_data)
+            case ReceviedAttesttionShare(attestation_share) => 
+                f_listen_for_attestation_shares.requires(s, attestation_share)
+            case ImportedNewBlock(block) => 
+                f_listen_for_new_imported_blocks.requires(s, block)
+            case ResendAttestationShares => 
+                f_resend_attestation_share.requires(s) 
+            case NoEvent => 
+                true
+    {
+        match event 
+            case ServeAttstationDuty(attestation_duty) => 
+                f_serve_attestation_duty(s, attestation_duty)
+            case AttConsensusDecided(id, decided_attestation_data) => 
+                f_att_consensus_decided(s, id,  decided_attestation_data)
+            case ReceviedAttesttionShare(attestation_share) => 
+                f_listen_for_attestation_shares(s, attestation_share)
+            case ImportedNewBlock(block) => 
+                f_listen_for_new_imported_blocks(s, block)
+            case ResendAttestationShares => 
+                f_resend_attestation_share(s)
+            case NoEvent => 
+                DVCNodeStateAndOuputs(state := s, outputs := getEmptyOuputs() )
+    }    
+
     function f_serve_attestation_duty(
         process: DVCNodeState,
         attestation_duty: AttestationDuty
     ): DVCNodeStateAndOuputs
+    requires forall ad | ad in process.attestation_duties_queue + [attestation_duty]:: ad.slot !in process.attestation_consensus_engine_state.attestation_consensus_active_instances.Keys
     {
         f_check_for_next_queued_duty(
             process.(
@@ -185,6 +323,7 @@ abstract module DVCNode_Spec {
     }    
 
     function f_check_for_next_queued_duty(process: DVCNodeState): DVCNodeStateAndOuputs
+    requires forall ad | ad in process.attestation_duties_queue :: ad.slot !in process.attestation_consensus_engine_state.attestation_consensus_active_instances.Keys
     decreases process.attestation_duties_queue
     {
         if  && process.attestation_duties_queue != [] 
@@ -213,16 +352,26 @@ abstract module DVCNode_Spec {
     }         
 
     function f_start_next_duty(process: DVCNodeState, attestation_duty: AttestationDuty): DVCNodeStateAndOuputs
+    requires attestation_duty.slot !in process.attestation_consensus_engine_state.attestation_consensus_active_instances.Keys
     {
+        var validityPredicate := 
+                (ad: AttestationData)  => 
+                    consensus_is_valid_attestation_data(process.attestation_slashing_db, ad, attestation_duty)
+                ;        
         DVCNodeStateAndOuputs(
             state :=  process.(
                         attestation_shares_db := map[],
-                        attestation_share_to_broadcast := None,
-                        current_attesation_duty := Some(attestation_duty)
+                        // attestation_shares_to_broadcast := None,
+                        current_attesation_duty := Some(attestation_duty),
+                        latest_attestation_duty := Some(attestation_duty),
+                        attestation_consensus_engine_state := startConsensusInstance(
+                            process.attestation_consensus_engine_state,
+                            attestation_duty.slot,
+                            attestation_duty,
+                            process.attestation_slashing_db
+                        )
             ),
-            outputs := getEmptyOuputs().(
-                att_consensus_commands_sent := {ConsensusCommand.Start(attestation_duty.slot)}
-            )
+            outputs := getEmptyOuputs()
         )        
     }      
 
@@ -252,6 +401,7 @@ abstract module DVCNode_Spec {
         decided_attestation_data: AttestationData
     ): DVCNodeStateAndOuputs
     requires process.current_attesation_duty.isPresent()
+    requires forall ad | ad in process.attestation_duties_queue :: ad.slot !in process.attestation_consensus_engine_state.attestation_consensus_active_instances.Keys    
     {
         var local_current_attestation_duty := process.current_attesation_duty.safe_get();
         var attestation_slashing_db := f_update_attestation_slashing_db(process.attestation_slashing_db, decided_attestation_data, local_current_attestation_duty.pubkey);
@@ -263,17 +413,76 @@ abstract module DVCNode_Spec {
         var attestation_with_signature_share := AttestationShare(
                 aggregation_bits := get_aggregation_bits(local_current_attestation_duty.validator_index),
                 data := decided_attestation_data, 
-                signature :=attestation_signature_share
+                signature := attestation_signature_share
             ); 
 
-        DVCNodeStateAndOuputs(
-            state := process.(
-                attestation_share_to_broadcast := Some(attestation_with_signature_share)
-            ),
+        var newProcess := 
+            process.(
+                current_attesation_duty := None,
+                attestation_shares_to_broadcast := process.attestation_shares_to_broadcast[local_current_attestation_duty.slot := attestation_with_signature_share],
+                attestation_slashing_db := attestation_slashing_db,
+                attestation_consensus_engine_state := updateConsensusInstanceValidityCheck(
+                    process.attestation_consensus_engine_state,
+                    attestation_slashing_db
+                )
+            );
+
+        // DVCNodeStateAndOuputs(
+        //     newProcess,
+        //     outputs := getEmptyOuputs().(
+        //         att_shares_sent := multicast(attestation_with_signature_share, process.peers)
+        //     )                  
+        // )
+
+        // newProcess       
+
+        var ret_check_for_next_queued_duty := f_check_for_next_queued_duty(newProcess);
+
+        ret_check_for_next_queued_duty.(
+            state := ret_check_for_next_queued_duty.state,
             outputs := getEmptyOuputs().(
                 att_shares_sent := multicast(attestation_with_signature_share, process.peers)
-            )
-        )         
+            )          
+        )
+
+
+        // if newProces.current_attesation_duty.isPresent() && newProces.current_attesation_duty.safe_get().slot in newProces.future_att_consensus_instances_already_decided then
+        //     // Stop(current_attesation_duty.safe_get().slot);
+        //     var newProces2 := newProces.(
+        //         current_attesation_duty := None,
+        //         attestation_consensus_engine_state := stopConsensusInstances(
+        //                     newProces.attestation_consensus_engine_state,
+        //                     newProces.current_attesation_duty.safe_get().slot
+        //                 )
+        //     );
+        //     var r := f_check_for_next_queued_duty(newProces2);
+        //     r
+        //     // DVCNodeStateAndOuputs(
+        //     //     state := r.state,
+        //     //     outputs := getEmptyOuputs()
+        //     //     // r.outputs.(
+        //     //     //     att_consensus_commands_sent := r.outputs.att_consensus_commands_sent + {ConsensusCommand.Stop(process.current_attesation_duty.safe_get().slot)}
+        //     //     // )
+        //     // )
+        // else
+        //     DVCNodeStateAndOuputs(
+        //         state := newProces,
+        //         outputs := getEmptyOuputs()
+        //     )            
+
+        // DVCNodeStateAndOuputs(
+        //     state := process.(
+        //         attestation_shares_to_broadcast := process.attestation_shares_to_broadcast[local_current_attestation_duty.slot := attestation_with_signature_share],
+        //         attestation_slashing_db := attestation_slashing_db,
+        //         attestation_consensus_engine_state := updateConsensusInstanceValidityCheck(
+        //             process.attestation_consensus_engine_state,
+        //             attestation_slashing_db
+        //         )
+        //     ),
+        //     outputs := getEmptyOuputs().(
+        //         att_shares_sent := multicast(attestation_with_signature_share, process.peers)
+        //     )
+        // )         
     }    
 
     function f_listen_for_attestation_shares(
@@ -328,7 +537,7 @@ abstract module DVCNode_Spec {
             && var i:nat :| i < |committee| && committee[i] == valIndex.v;
             && i < |a.aggregation_bits|
             && a.aggregation_bits[i]
-            && (process.current_attesation_duty.isPresent() ==> a.data.slot >= process.current_attesation_duty.safe_get().slot)            
+            // && (process.current_attesation_duty.isPresent() ==> a.data.slot >= process.current_attesation_duty.safe_get().slot)            
     }
 
     function f_listen_for_new_imported_blocks(
@@ -345,24 +554,53 @@ abstract module DVCNode_Spec {
             ::
                 a.data.slot;
 
-        var newProces := process.(
-            future_att_consensus_instances_already_decided := process.future_att_consensus_instances_already_decided + s
-        );
+        var att_consensus_instances_already_decided := process.future_att_consensus_instances_already_decided + s;
 
-        if process.current_attesation_duty.isPresent() && process.current_attesation_duty.safe_get().slot in process.future_att_consensus_instances_already_decided then
-            // Stop(current_attesation_duty.safe_get().slot);
-            var r := f_check_for_next_queued_duty(newProces);
-            DVCNodeStateAndOuputs(
-                state := r.state,
-                outputs := r.outputs.(
-                    att_consensus_commands_sent := r.outputs.att_consensus_commands_sent + {ConsensusCommand.Stop(process.current_attesation_duty.safe_get().slot)}
-                )
-            )
-        else
-            DVCNodeStateAndOuputs(
-                state := newProces,
-                outputs := getEmptyOuputs()
-            )
+        var future_att_consensus_instances_already_decided := 
+                if process.latest_attestation_duty.isPresent() then
+                        set i | 
+                            && i in att_consensus_instances_already_decided 
+                            && i > process.latest_attestation_duty.safe_get().slot
+                else
+                    att_consensus_instances_already_decided
+                        ;
+
+        DVCNodeStateAndOuputs(
+            state :=
+                process.(
+                    future_att_consensus_instances_already_decided := future_att_consensus_instances_already_decided,
+                    attestation_consensus_engine_state := stopConsensusInstances(
+                                    process.attestation_consensus_engine_state,
+                                    att_consensus_instances_already_decided
+                    ),
+                    attestation_shares_to_broadcast := process.attestation_shares_to_broadcast - att_consensus_instances_already_decided
+                ),
+            outputs := getEmptyOuputs()
+        )
+
+        // if newProces.current_attesation_duty.isPresent() && newProces.current_attesation_duty.safe_get().slot in newProces.future_att_consensus_instances_already_decided then
+        //     // Stop(current_attesation_duty.safe_get().slot);
+        //     var newProces2 := newProces.(
+        //         current_attesation_duty := None,
+        //         attestation_consensus_engine_state := stopConsensusInstances(
+        //                     newProces.attestation_consensus_engine_state,
+        //                     newProces.current_attesation_duty.safe_get().slot
+        //                 )
+        //     );
+        //     var r := f_check_for_next_queued_duty(newProces2);
+        //     r
+        //     // DVCNodeStateAndOuputs(
+        //     //     state := r.state,
+        //     //     outputs := getEmptyOuputs()
+        //     //     // r.outputs.(
+        //     //     //     att_consensus_commands_sent := r.outputs.att_consensus_commands_sent + {ConsensusCommand.Stop(process.current_attesation_duty.safe_get().slot)}
+        //     //     // )
+        //     // )
+        // else
+        //     DVCNodeStateAndOuputs(
+        //         state := newProces,
+        //         outputs := getEmptyOuputs()
+        //     )
     }    
   
     function f_resend_attestation_share(
@@ -373,17 +611,14 @@ abstract module DVCNode_Spec {
             state := process,
             outputs := getEmptyOuputs().(
                 att_shares_sent :=
-                    if process.attestation_share_to_broadcast.isPresent() then
-                        multicast(process.attestation_share_to_broadcast.safe_get(), process.peers)
-                    else
-                        {}
-                    )
+                    multicast_multiple(process.attestation_shares_to_broadcast.Values, process.peers)
+            )
         )
 
     }        
 }
 
-abstract module DVCNode_Externs_Proofs refines DVCNode_Externs
+module DVCNode_Externs_Proofs refines DVCNode_Externs
 {
     import opened DVCNode_Spec
 
@@ -395,7 +630,7 @@ abstract module DVCNode_Externs_Proofs refines DVCNode_Externs
         )
     }
 
-    class BeaconNode...
+    trait BeaconNode...
     {
         method get_fork_version...
         ensures bn_get_fork_version(s) == v
@@ -408,7 +643,7 @@ abstract module DVCNode_Externs_Proofs refines DVCNode_Externs
     }
 
 
-    class RemoteSigner...
+    trait RemoteSigner...
     {
         method sign_attestation...
         ensures rs_sign_attestation(attestation_data, fork_version, signing_root, toRSState(this)) == s
