src/dvspec/dafny/specification/consensus.dfy
@@ -5,19 +5,20 @@ module ConsensusSpec
 {
     import opened Types 
 
-    datatype InCommand = 
+    datatype InCommand<!D> = 
     | Start(node: BLSPubkey)
     | Stop(node: BLSPubkey)
 
     datatype OutCommand<D> = 
     | Decided(node: BLSPubkey, value: D)
 
-    datatype HonestNodeStatus = NEVER_STARTED | STARTED | DECIDED | STOPPED
+    datatype HonestNodeStatus = NOT_DECIDED | DECIDED
 
-    datatype ConsensusInstance<D(!new, 0)> = ConsensusInstance(
+    datatype ConsensusInstance<!D(!new, 0)> = ConsensusInstance(
         all_nodes: set<BLSPubkey>,
         decided_value: Optional<D>,
-        honest_nodes_status: map<BLSPubkey, HonestNodeStatus>
+        honest_nodes_status: map<BLSPubkey, HonestNodeStatus>,
+        ghost honest_nodes_validity_functions: set<D -> bool>
     )    
 
 
@@ -30,14 +31,14 @@ module ConsensusSpec
     function quorum(n:nat):nat
     // returns ceil(2n/3)
 
-    function getRunningNodes<D(!new, 0)>(
-        s: ConsensusInstance
-    ): set<BLSPubkey> 
-    {
-        set n | 
-            && n in s.honest_nodes_status
-            && s.honest_nodes_status[n] in {STARTED, DECIDED}
-    }
+    // function getRunningNodes<D(!new, 0)>(
+    //     s: ConsensusInstance
+    // ): set<BLSPubkey> 
+    // {
+    //     set n | 
+    //         && n in s.honest_nodes_status
+    //         && s.honest_nodes_status[n] in {STARTED, DECIDED}
+    // }
 
     predicate isConditionForSafetyTrue<D(!new, 0)>(
         s: ConsensusInstance
@@ -46,14 +47,14 @@ module ConsensusSpec
         quorum(|s.all_nodes|) <= |s.honest_nodes_status|
     }
 
-    predicate isNodeRunning<D(!new, 0)>(
-        s: ConsensusInstance,
-        node: BLSPubkey
-    )
-    {
-        && node in s.honest_nodes_status.Keys
-        && s.honest_nodes_status[node] in {STARTED, DECIDED}
-    }
+    // predicate isNodeRunning<D(!new, 0)>(
+    //     s: ConsensusInstance,
+    //     node: BLSPubkey
+    // )
+    // {
+    //     && node in s.honest_nodes_status.Keys
+    //     && s.honest_nodes_status[node] in {STARTED, DECIDED}
+    // }
 
     predicate Init<D(!new, 0)>(
         s: ConsensusInstance, 
@@ -63,62 +64,64 @@ module ConsensusSpec
         && s.all_nodes == all_nodes
         && !s.decided_value.isPresent()
         && s.honest_nodes_status.Keys == honest_nodes
-        && forall t | t in s.honest_nodes_status.Values :: t == NEVER_STARTED
+        && forall t | t in s.honest_nodes_status.Values :: t == NOT_DECIDED
     }
 
     predicate Next<D(!new, 0)>(
         s: ConsensusInstance,
-        input: Optional<InCommand>,
-        validityPredicate: D -> bool,
+        // input: Optional<InCommand>,
+        honest_nodes_validity_predicates: map<BLSPubkey, D -> bool>,        
         s': ConsensusInstance,
         output: Optional<OutCommand>
     )
     {
         exists s'': ConsensusInstance ::
             // First we let the consensus protocol and the various nodes possibly decide on a value
-            && NextConsensusDecides(s, validityPredicate, s'')
+            && NextConsensusDecides(s, honest_nodes_validity_predicates, s'')
             // Then we let the node take an input/output step
-            && NextNodeStep(s'', input, s', output)
+            && NextNodeStep(s'', honest_nodes_validity_predicates, s', output)
 
     }
 
     predicate NextNodeStep<D(!new, 0)>(
         s: ConsensusInstance,
-        input: Optional<InCommand>,
+        honest_nodes_validity_predicates: map<BLSPubkey, D -> bool>,
         s': ConsensusInstance,
         output: Optional<OutCommand>
     )
     {
         && (
-            || (
-                && input.isPresent()
-                && !output.isPresent()
-                && input.safe_get().Start?
-                && var n := input.safe_get().node;
-                && n in s.honest_nodes_status.Keys 
-                && s.honest_nodes_status[n] in {NEVER_STARTED, STARTED}
-                && s' == s.(
-                    honest_nodes_status := s.honest_nodes_status[n := STARTED]
-                )
+            // || (
+            //     && input.isPresent()
+            //     && !output.isPresent()
+            //     && input.safe_get().Start?
+            //     && var n := input.safe_get().node;
+            //     && n in s.honest_nodes_status.Keys 
+            //     && s.honest_nodes_status[n] in {NEVER_STARTED, STARTED}
+            //     && s' == s.(
+            //         honest_nodes_status := s.honest_nodes_status[n := STARTED]
+            //     )
                 
-            )
-            || (
-                && input.isPresent()
-                && !output.isPresent()
-                && input.safe_get().Stop?
-                && var n := input.safe_get().node;
-                && n in s.honest_nodes_status.Keys 
-                && s.honest_nodes_status[n] == STARTED
-                && s' == s.(
-                    honest_nodes_status := s.honest_nodes_status[n := STOPPED]
-                )
+            // )
+            // || (
+            //     && input.isPresent()
+            //     && !output.isPresent()
+            //     && input.safe_get().Stop?
+            //     && var n := input.safe_get().node;
+            //     && n in s.honest_nodes_status.Keys 
+            //     && s.honest_nodes_status[n] == STARTED
+            //     && s' == s.(
+            //         honest_nodes_status := s.honest_nodes_status[n := STOPPED]
+            //     )
                 
-            )    
-            || (
-                && !input.isPresent()
+            // )    
+            // || 
+            (
+                // && !input.isPresent()
                 && output.isPresent()
                 && var n := output.safe_get().node;
                 && n in s.honest_nodes_status.Keys 
+                && n in honest_nodes_validity_predicates.Keys
                 && s.honest_nodes_status[n] in {DECIDED}
                 &&  if isConditionForSafetyTrue(s) then
                         && s.decided_value.isPresent()
@@ -133,21 +136,22 @@ module ConsensusSpec
 
     predicate NextConsensusDecides<D(!new, 0)>(
         s: ConsensusInstance,
-        validityPredicate: D -> bool,
+        honest_nodes_validity_predicates: map<BLSPubkey, D -> bool>,    
         s': ConsensusInstance
     )
     {
+        && s'.honest_nodes_validity_functions == s.honest_nodes_validity_functions + honest_nodes_validity_predicates.Values
         && (
             || (
                 && (isConditionForSafetyTrue(s) ==>
                                                     && s'.decided_value.isPresent()
                                                     && (s.decided_value.isPresent() ==> s'.decided_value == s.decided_value)
-                                                    && validityPredicate(s'.decided_value.safe_get())
+                                                    && (exists vp | vp in s'.honest_nodes_validity_functions :: vp(s'.decided_value.safe_get()))
                 )
                 && s'.honest_nodes_status.Keys == s.honest_nodes_status.Keys
                 && forall n | n in s.honest_nodes_status.Keys ::
-                    if s.honest_nodes_status[n] == STARTED then 
-                        s'.honest_nodes_status[n] in {STARTED, DECIDED}
+                    if n in honest_nodes_validity_predicates then 
+                        s.honest_nodes_status[n] == DECIDED ==> s'.honest_nodes_status[n] == DECIDED
                     else 
                         s'.honest_nodes_status[n] == s.honest_nodes_status[n]
                 && s'.all_nodes == s.all_nodes
