src/dvspec/dafny/specification/dvn.dfy
@@ -27,7 +27,7 @@ abstract module DV
         consensus_on_attestation_data: imaptotal<Slot, ConsensusInstance<AttestationData>>,
         att_network: NetworkSpec.Network<AttestationShare>,
         all_attestations_created: set<Attestation>,
-        slashing_dbs_used_for_validating_attestations: imaptotal<Slot, set<AttestationSlashingDB>>,
+        // slashing_dbs_used_for_validating_attestations: imaptotal<Slot, set<AttestationSlashingDB>>,
         // aggregated_attestations_sent: set<Attestation>,
         // attestation_duties_served: map<AttestationDuty, set<BLSPubkey>>,
         construct_signed_attestation_signature: (set<AttestationShare>) -> Optional<BLSSignature>
@@ -84,7 +84,7 @@ abstract module DV
 
         )   
         && s.all_attestations_created == {}
-        && s.slashing_dbs_used_for_validating_attestations == (imap s: Slot :: {})   
+        // && s.slashing_dbs_used_for_validating_attestations == (imap s: Slot :: {})   
         && (
             forall n | n in s.honest_nodes_states.Keys ::
                 DVCNode_Spec.Init(s.honest_nodes_states[n], s.dv_pubkey, s.all_nodes, s.construct_signed_attestation_signature)
@@ -178,29 +178,29 @@ abstract module DV
                 case _ => {}
             ;
         && NetworkSpec.Next(s.att_network, s'.att_network, node, nodeOutputs.att_shares_sent, messagesReceivedByTheNode)
-        && (
-                forall consensus_id: Slot ::
-                    s'.slashing_dbs_used_for_validating_attestations[consensus_id] == s.slashing_dbs_used_for_validating_attestations[consensus_id] +
-                        if isNodeRunning(s.consensus_on_attestation_data[consensus_id], node) then
-                            {s'.honest_nodes_states[node].attestation_slashing_db}
-                        else
-                            {}
-            )
+        // && (
+        //         forall consensus_id: Slot ::
+        //             s'.slashing_dbs_used_for_validating_attestations[consensus_id] == s.slashing_dbs_used_for_validating_attestations[consensus_id] +
+        //                 if isNodeRunning(s.consensus_on_attestation_data[consensus_id], node) then
+        //                     {s'.honest_nodes_states[node].attestation_slashing_db}
+        //                 else
+        //                     {}
+        //     )
         && (
             forall cid | cid in s.consensus_on_attestation_data.Keys ::
-                var inputCommands := set c | 
-                                    && c in nodeOutputs.att_consensus_commands_sent
-                                    && c.id == cid
-                            ::
-                                if c.Start? then 
-                                    Some(ConsensusSpec.Start(node))
-                                else
-                                    Some(ConsensusSpec.Stop(node));
-                var input :|
-                    if inputCommands == {} then
-                        input == None
-                    else
-                        input in inputCommands;
+                // var inputCommands := set c | 
+                //                     && c in nodeOutputs.att_consensus_commands_sent
+                //                     && c.id == cid
+                //             ::
+                //                 if c.Start? then 
+                //                     Some(ConsensusSpec.Start(node))
+                //                 else
+                //                     Some(ConsensusSpec.Stop(node));
+                // var input :|
+                //     if inputCommands == {} then
+                //         input == None
+                //     else
+                //         input in inputCommands;
 
                 var output := 
                     if nodeEvent.AttConsensusDecided? && nodeEvent.id == cid then 
@@ -212,29 +212,30 @@ abstract module DV
                 // The consenus protocol is exepcted to decide on an attestation data such that there exists at least one slashing_db, out of 
                 // the slashing_dbs that any honest node has had while participating in the consenus, for which the attestation data does not
                 // generate any slashabe condition.
-                && var validityPredicate := 
-                    (ad: AttestationData) => 
-                        exists db | db in s.slashing_dbs_used_for_validating_attestations[cid] ::
-                            !is_slashable_attestation(db, ad)
+                && var validityPredicates := 
+                    map n |
+                            && n in s.honest_nodes_states.Keys 
+                            && cid in s.honest_nodes_states[n].attestation_consensus_engine_state.attestation_consensus_active_instances.Keys
+                        ::
+                            s.honest_nodes_states[n].attestation_consensus_engine_state.attestation_consensus_active_instances[cid].validityPredicate
                     ;
 
                 ConsensusSpec.Next(
                     s.consensus_on_attestation_data[cid],
-                    input,
-                    validityPredicate,
+                    validityPredicates,
                     s'.consensus_on_attestation_data[cid],
                     output
                 )
         )
-        && (
-            // This section collects all the slashing_dbs used by honest nodes participating in the various consensus instances
-            forall consensus_id: Slot ::
-                s'.slashing_dbs_used_for_validating_attestations[consensus_id] == s.slashing_dbs_used_for_validating_attestations[consensus_id] +
-                    if node in getRunningNodes(s'.consensus_on_attestation_data[consensus_id]) then
-                        {s'.honest_nodes_states[node].attestation_slashing_db}
-                    else
-                        {}
-        )        
+        // && (
+        //     // This section collects all the slashing_dbs used by honest nodes participating in the various consensus instances
+        //     forall consensus_id: Slot ::
+        //         s'.slashing_dbs_used_for_validating_attestations[consensus_id] == s.slashing_dbs_used_for_validating_attestations[consensus_id] +
+        //             if node in getRunningNodes(s'.consensus_on_attestation_data[consensus_id]) then
+        //                 {s'.honest_nodes_states[node].attestation_slashing_db}
+        //             else
+        //                 {}
+        // )        
         && s'.adversary == s.adversary
         && s'.construct_signed_attestation_signature == s.construct_signed_attestation_signature
     }    
